cryptis/primitives/pre_term.v
@@ -16,29 +16,60 @@ Set Implicit Arguments.
 Unset Strict Implicit.
 Unset Printing Implicit Defensive.
 
+Definition eq_term_op0 : val := λ: "x" "y",
+  (Fst "x" = Fst "y") && (Snd "x" = Snd "y").
+
+Definition eq_key_type : val := λ: "x" "y",
+  "x" = "y".
+
+Definition eq_term_op1 : val := λ: "x" "y",
+  if: (Fst "x" = Fst "y") then
+    let: "tag" := Fst "x" in
+    if: "tag" = #0 (* Key *) then
+      eq_key_type (Snd "x") (Snd "y")
+    else (* Hash *) #true
+  else #false.
+
+Definition eq_term_op2 : val := λ: "x" "y",
+  "x" = "y".
+
 Definition eq_term : val := (rec: "eq" "x" "y" :=
   if: (Fst "x" = Fst "y") then
     let: "tag" := Fst "x" in
-    if: "tag" = #TInt_tag then
-      Snd "x" = Snd "y"
-    else if: "tag" = #TPair_tag then
-      ("eq" (Fst (Snd "x")) (Fst (Snd "y"))) &&
-      ("eq" (Snd (Snd "x")) (Snd (Snd "y")))
-    else if: "tag" = #TNonce_tag then
-      Snd "x" = Snd "y"
-    else if: "tag" = #TKey_tag then
-      (Fst (Snd "x") = Fst (Snd "y")) &&
+    if: "tag" = #TOp0_tag then
+      eq_term_op0 (Snd "x") (Snd "y")
+    else if: "tag" = #TOp1_tag then
+      eq_term_op1 (Fst (Snd "x")) (Fst (Snd "y")) &&
       "eq" (Snd (Snd "x")) (Snd (Snd "y"))
-    else if: "tag" = #TSeal_tag then
-      "eq" (Fst (Snd "x")) (Fst (Snd "y")) &&
+    else if: "tag" = #TOp2_tag then
+      eq_term_op2 (Fst (Fst (Snd "x"))) (Fst (Fst (Snd "y"))) &&
+      "eq" (Snd (Fst (Snd "x"))) (Snd (Fst (Snd "y"))) &&
       "eq" (Snd (Snd "x")) (Snd (Snd "y"))
-    else if: "tag" = #THash_tag then
-      "eq" (Snd "x") (Snd "y")
     else if: "tag" = #TExp_tag then
       "eq" (Fst (Snd "x")) (Fst (Snd "y")) &&
       eq_list "eq" (Snd (Snd "x")) (Snd (Snd "y"))
     else #false
   else #false)%V.
+
+Definition leq_term_op0 : val := λ: "x" "y",
+  if: (Fst "x" < Fst "y") then #true
+  else if: (Fst "x" = Fst "y") then
+    if: Fst "x" = #0 (* Int *) then Snd "x" ≤ Snd "y"
+    else leq_loc (Snd "x") (Snd "y") (* Nonce *)
+  else #false.
+
+Definition leq_key_type : val := λ: "x" "y",
+  "x" ≤ "y".
+
+Definition leq_term_op1 : val := λ: "x" "y",
+  if: (Fst "x" < Fst "y") then #true
+  else if: (Fst "x" = Fst "y") then
+    if: Fst "x" = #0 (* Key *) then leq_key_type (Snd "x") (Snd "y")
+    else #true (* Hash *)
+  else #false.
+
+Definition leq_term_op2 : val := λ: "x" "y",
+  "x" ≤ "y".
 
 Definition leq_term : val := rec: "loop" "t1" "t2" :=
  (if: (Fst "t1" < Fst "t2") then #true
@@ -46,32 +77,28 @@ Definition leq_term : val := rec: "loop" "t1" "t2" :=
     let: "tag" := Fst "t1" in
     let: "a1"  := Snd "t1" in
     let: "a2"  := Snd "t2" in
-    if: "tag" = #TInt_tag then "a1" ≤ "a2"
-    else if: "tag" = #TPair_tag then
-      let: "t11" := Fst "a1" in
+    if: "tag" = #TOp0_tag then
+      let: "o1" := "a1" in
+      let: "o2" := "a2" in
+      leq_term_op0 "o1" "o2"
+    else if: "tag" = #TOp1_tag then
+      let: "o1" := Fst "a1" in
+      let: "t1" := Snd "a1" in
+      let: "o2" := Fst "a2" in
+      let: "t2" := Snd "a2" in
+      if: eq_term_op1 "o1" "o2" then "loop" "t1" "t2"
+      else leq_term_op1 "o1" "o2"
+    else if: "tag" = #TOp2_tag then
+      let: "o1" := Fst (Fst "a1") in
+      let: "t11" := Snd (Fst "a1") in
       let: "t12" := Snd "a1" in
-      let: "t21" := Fst "a2" in
+      let: "o2" := Fst (Fst "a2") in
+      let: "t21" := Snd (Fst "a2") in
       let: "t22" := Snd "a2" in
-      if: eq_term "t11" "t21" then "loop" "t12" "t22"
-      else "loop" "t11" "t21"
-    else if: "tag" = #TNonce_tag then
-      leq_loc "a1" "a2"
-    else if: "tag" = #TKey_tag then
-      let: "kt1" := Fst "a1" in
-      let: "t1"  := Snd "a1" in
-      let: "kt2" := Fst "a2" in
-      let: "t2"  := Snd "a2" in
-      if: "kt1" = "kt2" then "loop" "t1" "t2"
-      else "kt1" ≤ "kt2"
-    else if: "tag" = #TSeal_tag then
-      let: "t11" := Fst "a1" in
-      let: "t12" := Snd "a1" in
-      let: "t21" := Fst "a2" in
-      let: "t22" := Snd "a2" in
-      if: eq_term "t11" "t21" then "loop" "t12" "t22"
-      else "loop" "t11" "t21"
-    else if: "tag" = #THash_tag then
-      "loop" "a1" "a2"
+      if: eq_term_op2 "o1" "o2" then
+        if: eq_term "t11" "t21" then "loop" "t12" "t22"
+        else "loop" "t11" "t21"
+      else leq_term_op2 "o1" "o2"
     else if: "tag" = #TExp_tag then
       let: "t1" := Fst "a1" in
       let: "ts1" := Snd "a1" in
@@ -102,49 +129,77 @@ Implicit Types v : val.
 Implicit Types Ψ : val → iProp Σ.
 Implicit Types N : namespace.
 
+Lemma twp_eq_term_op0 E (o1 o2 : term_op0) :
+  ⊢ WP (eq_term_op0 (repr o1) (repr o2)) @ E
+    [{ v, ⌜v = #(bool_decide (o1 = o2))⌝}].
+Proof.
+case: o1 o2 => [n1|a1] [n2|a2] /=; wp_lam; wp_pures => //.
+- iPureIntro. congr (# (LitBool _)). apply: bool_decide_ext.
+  intuition congruence.
+- iPureIntro. congr (# (LitBool _)). apply: bool_decide_ext.
+  intuition congruence.
+Qed.
+
+Lemma twp_eq_key_type E (o1 o2 : key_type) :
+  ⊢ WP (eq_key_type (repr o1) (repr o2)) @ E
+    [{ v, ⌜v = #(bool_decide (o1 = o2))⌝}].
+Proof.
+case: o1 o2 => [] [] /=; wp_lam; wp_pures => //.
+Qed.
+
+Lemma twp_eq_term_op1 E (o1 o2 : term_op1) :
+  ⊢ WP (eq_term_op1 (repr o1) (repr o2)) @ E
+    [{ v, ⌜v = #(bool_decide (o1 = o2))⌝}].
+Proof.
+case: o1 o2 => [o1|] [o2|] /=; wp_lam; wp_pures => //.
+iApply twp_wand; first wp_apply twp_eq_key_type.
+iIntros (?) "->". iPureIntro.
+congr (# (LitBool _)). apply: bool_decide_ext.
+intuition congruence.
+Qed.
+
+Lemma twp_eq_term_op2 E (o1 o2 : term_op2) :
+  ⊢ WP (eq_term_op2 (repr o1) (repr o2)) @ E
+    [{ v, ⌜v = #(bool_decide (o1 = o2))⌝}].
+Proof.
+case: o1 o2 => [] [] /=; wp_lam; wp_pures => //.
+Qed.
+
 Lemma twp_eq_pre_term_aux E (pt1 pt2 : PreTerm.pre_term) :
   ⊢ WP (eq_term (repr pt1) (repr pt2)) @ E
        [{ v, ⌜v = #(bool_decide (pt1 = pt2))⌝ }].
 Proof.
-rewrite /= val_of_pre_term_unseal.
-elim: pt1 pt2
-  => [n1|t11 IH1 t12 IH2|l1|kt1 t1 IH1|t11 IH1 t12 IH2|t1 IH|t1 IHt1 ts1 IHts1];
-case=> [n2|t21 t22|l2|kt2 t2|t21 t22|t2|t2 ts2] /=;
-wp_rec; wp_pures=> //.
-- iPureIntro; congr (# (LitBool _)).
+elim: pt1 pt2 => [o1|o1 t1 IH1|o1 t11 IH1 t12 IH2|t1 IHt1 ts1 IHts1];
+case=> [o2|o2 t2|o2 t21 t22|t2 ts2]; wp_rec; wp_pures=> //.
+- iApply twp_wand; first by wp_apply twp_eq_term_op0.
+  iIntros (?) "->". iPureIntro; congr (# (LitBool _)).
   apply: bool_decide_ext; intuition congruence.
-- wp_bind (eq_term _ _).
-  iPoseProof (IH1 t21) as "IH1"; iPoseProof (IH2 t22) as "IH2".
-  iApply (twp_wand with "IH1"); iIntros (?) "->".
-  case: bool_decide_reflect=> e1.
-  + wp_pures; iApply (twp_wand with "IH2"); iIntros (?) "->".
-    iPureIntro; congr (# (LitBool _)).
+- wp_bind (eq_term_op1 _ _).
+  iApply twp_wand; first by wp_apply twp_eq_term_op1.
+  iIntros (?) "->". case: bool_decide_reflect=> e1.
+  + wp_pures. iApply twp_wand; first by wp_apply IH1.
+    iIntros (?) "->". iPureIntro; congr (# (LitBool _)).
     apply: bool_decide_ext; intuition congruence.
   + wp_pures; iPureIntro; congr (# (LitBool _)).
     rewrite bool_decide_false; congruence.
-- iPureIntro; congr (# (LitBool _)).
-  apply: bool_decide_ext; intuition congruence.
-- case: bool_decide_reflect=> [[/int_of_key_type_inj e1]|e1].
-  + wp_pures; iApply twp_wand; first iApply IH1.
-    iPureIntro => _ ->; congr (# (LitBool _)).
-    apply: bool_decide_ext; intuition congruence.
-  + wp_pures; iPureIntro; congr (# (LitBool _)).
+- wp_bind (eq_term_op2 _ _).
+  iApply twp_wand; first by wp_apply twp_eq_term_op2.
+  iIntros (?) "->". case: bool_decide_reflect=> e1; last first.
+    wp_pures; iPureIntro; congr (# (LitBool _)).
     rewrite bool_decide_false; congruence.
-- wp_pures; wp_bind (eq_term _ _); iApply twp_wand; first iApply IH1.
-  iIntros (?) "->"; case: bool_decide_reflect=> e1; wp_pures; last first.
-    iPureIntro; rewrite bool_decide_false //; congruence.
-  iApply twp_wand; first iApply IH2.
-  iIntros (?) "->"; case: bool_decide_reflect=> e2; last first.
-    rewrite bool_decide_false //; congruence.
-  iPureIntro; congr (# (LitBool _)).
-  by rewrite bool_decide_true //; congruence.
-- wp_pures; iApply twp_wand; first iApply IH.
-  iIntros (?) "->"; iPureIntro; congr (# (LitBool _)).
-  apply: bool_decide_ext; intuition congruence.
+  wp_pures. wp_bind (eq_term _ _).
+  wp_apply twp_wand; first by wp_apply IH1.
+  iIntros (?) "->". case: bool_decide_reflect=> e2.
+    wp_pures. wp_bind (eq_term _ _).
+    wp_apply twp_wand; first by wp_apply IH2.
+    iIntros (?) "->". iPureIntro; congr (# (LitBool _)).
+    by apply: bool_decide_ext; intuition congruence.
+  wp_pures; iPureIntro; congr (# (LitBool _)).
+  rewrite bool_decide_false; congruence.
 - wp_bind (eq_term _ _); iApply twp_wand; first iApply IHt1.
   iIntros (?) "->"; case: bool_decide_reflect=> e1; wp_pures; last first.
     rewrite bool_decide_false //; congruence.
-  rewrite -val_of_pre_term_unseal -!repr_list_val.
+  rewrite -!repr_list_val.
   iApply (@twp_eq_list PreTerm.pre_term); last first.
     iPureIntro; congr (# (LitBool _)); apply: bool_decide_ext.
     rewrite e1; split; congruence.
@@ -154,7 +209,6 @@ wp_rec; wp_pures=> //.
   case=> IHx1 /IH IHts1 x1' x2' Ψ.
   rewrite elem_of_cons; case=> [->|x1'_in]; iIntros "post"; last first.
     by iApply IHts1.
-  rewrite -/val_of_pre_term val_of_pre_term_unseal.
   iApply twp_wand; first iApply IHx1; by iIntros (?) "->".
 Qed.
 
@@ -171,46 +225,66 @@ Import ssrbool seq path.
 
 Import ssreflect.eqtype ssreflect.order.
 
+Lemma twp_leq_term_op0 E (o1 o2 : term_op0) :
+  ⊢ WP (leq_term_op0 (repr o1) (repr o2)) @ E
+    [{ v, ⌜v = #(o1 <= o2)%O⌝}].
+Proof.
+rewrite PreTerm.op0_leqE.
+case: o1 o2 => [n1|a1] [n2|a2] /=; wp_lam; wp_pures => //.
+- iPureIntro. congr (# (LitBool _)). symmetry.
+  exact/(sameP (Z.leb_spec0 _ _))/bool_decide_reflect.
+- by iApply twp_leq_loc.
+Qed.
+
+Lemma twp_leq_term_op1 E (o1 o2 : term_op1) :
+  ⊢ WP (leq_term_op1 (repr o1) (repr o2)) @ E
+    [{ v, ⌜v = #(o1 <= o2)%O⌝}].
+Proof.
+rewrite PreTerm.op1_leqE.
+case: o1 o2 => [k1|] [k2|] /=; wp_lam; wp_pures => //.
+wp_lam; wp_pures. iPureIntro.
+by case: k1 k2 => [] [].
+Qed.
+
+Lemma twp_leq_term_op2 E (o1 o2 : term_op2) :
+  ⊢ WP (leq_term_op2 (repr o1) (repr o2)) @ E
+    [{ v, ⌜v = #(o1 <= o2)%O⌝}].
+Proof. by case: o1 o2 => [] [] /=; wp_lam; wp_pures => //. Qed.
+
 Lemma twp_leq_pre_term E (pt1 pt2 : PreTerm.pre_term) Ψ :
   Ψ #(pt1 <= pt2)%O ⊢
   WP (leq_term (repr pt1) (repr pt2)) @ E [{ Ψ }].
 Proof.
-rewrite /= val_of_pre_term_unseal.
-elim: pt1 pt2 Ψ
-  => [n1|t11 IH1 t12 IH2|l1|kt1 t1 IH1|t11 IH1 t12 IH2|t1 IH|t1 IHt1 ts1 IHts1];
-case=> [n2|t21 t22|l2|kt2 t2|t21 t22|t2|t2 ts2] /= Ψ;
+elim: pt1 pt2 Ψ => [o1|o1 t1 IH1|o1 t11 IH1 t12 IH2|t1 IHt1 ts1 IHts1];
+case => [o2|o2 t2|o2 t21 t22|t2 ts2] Ψ;
 iIntros "post"; wp_rec; wp_pures; try by iApply "post".
-- rewrite PreTerm.leqE /= (_ : (_ <= _)%O = bool_decide (n1 ≤ n2)%Z) //.
-  exact/(sameP (Z.leb_spec0 _ _))/bool_decide_reflect.
-- rewrite -{1 2}val_of_pre_term_unseal; wp_bind (eq_term _ _).
-  rewrite PreTerm.leqE /=; iApply twp_eq_pre_term.
-  rewrite eq_op_bool_decide; case: eqP => [->|_]; wp_pures.
-    by iApply IH2.
+- iApply twp_wand; first by wp_apply twp_leq_term_op0.
+  iIntros "% ->". by rewrite PreTerm.leqE.
+- rewrite PreTerm.leqE /=. wp_bind (eq_term_op1 _ _).
+  iApply twp_wand; first by wp_apply twp_eq_term_op1.
+  iIntros "% ->". rewrite eq_op_bool_decide.
+  case: (o1 == o2); wp_pures; first by iApply IH1.
+  iApply twp_wand. by iApply twp_leq_term_op1.
+  by iIntros "% ->".
+- rewrite PreTerm.leqE /=. wp_bind (eq_term_op2 _ _).
+  iApply twp_wand; first by wp_apply twp_eq_term_op2.
+  iIntros "% ->". rewrite eq_op_bool_decide.
+  case: (o1 == o2); wp_pures; last first.
+    iApply twp_wand. by iApply twp_leq_term_op2.
+    by iIntros "% ->".
+  wp_apply twp_eq_pre_term.
+  rewrite eq_op_bool_decide.
+  case: eq_op; wp_pures; first by iApply IH2.
   by iApply IH1.
-- by rewrite PreTerm.leqE /=; iApply twp_leq_loc.
-- rewrite PreTerm.leqE /=; case: eqP => [->|neq].
-    rewrite bool_decide_eq_true_2 //; wp_pures; by iApply IH1.
-  rewrite bool_decide_eq_false_2; last first.
-    move=> [e]; apply: neq.
-    by apply: int_of_key_type_inj.
-  wp_pures.
-  by case: kt1 kt2 {neq} => [] [].
 - rewrite PreTerm.leqE /=; wp_bind (eq_term _ _).
-  rewrite -{1 2}val_of_pre_term_unseal; iApply twp_eq_pre_term.
-  rewrite eq_op_bool_decide; case: eqP => [->|neq]; wp_pures.
-    by iApply IH2.
-  by iApply IH1.
-- rewrite PreTerm.leqE /=; by iApply IH.
-- rewrite PreTerm.leqE /=; wp_bind (eq_term _ _).
-  rewrite -{1 2}val_of_pre_term_unseal.
   iApply twp_eq_pre_term; rewrite eq_op_bool_decide.
   case: eqP=> [->|neq]; wp_pures; last by iApply IHt1.
-  rewrite -!repr_list_val -val_of_pre_term_unseal; iApply twp_leq_list => //.
+  rewrite -!repr_list_val; iApply twp_leq_list => //.
   + move=> pt1 pt2 Ψ'; iIntros "_ post".
     by iApply twp_eq_pre_term; rewrite eq_op_bool_decide; iApply "post".
   + move/foldr_in in IHts1.
     move=> ????; iIntros "_ post".
-    by rewrite /= val_of_pre_term_unseal; iApply IHts1 => //; iApply "post".
+    by rewrite /=; iApply IHts1 => //; iApply "post".
   + by iIntros "_".
 Qed.
 
